books/projects/rp-rewriter/lib/mult3/summation-tree-meta-fncs.lisp
@@ -56,6 +56,13 @@
 (local
  (in-theory (disable +-IS-SUM)))
 
+
+
+(define negated-termp (term)
+  :inline t
+  (case-match term (('-- &) t)))
+
+
 (progn
   (encapsulate
     (((stingy-pp-clean) => *))
@@ -75,9 +82,9 @@
 
   (enable-stingy-pp-clean t)
 
-  (define clean-pp-args-cond (s c-lst)
+  (define clean-pp-args-cond (s-lst c-lst)
     (or (not (stingy-pp-clean))
-        (and (equal s ''nil)
+        (and (equal s-lst nil)
              (or (atom c-lst)
                  (atom (cdr c-lst)))))))
 
@@ -94,9 +101,11 @@
   (b* ((c (ex-from-rp$ c)))
     (case-match c
       (('c ('quote hash-code) s pp ('list . c-lst))
-       (mv (ifix hash-code) s pp c-lst 'c))
+       (mv (if (consp hash-code) (ifix (car hash-code)) (ifix hash-code))
+           s pp c-lst 'c))
       (('c ('quote hash-code) s pp ''nil)
-       (mv (ifix hash-code) s pp nil 'c))
+       (mv (if (consp hash-code) (ifix (car hash-code)) (ifix hash-code))
+           s pp nil 'c))
       (& (mv 0 ''nil ''nil nil nil)))))
 
 (progn
@@ -157,24 +166,29 @@
 
   (defwarrant get-hash-code-of-single-s$inline)
 
-  (define get-hash-code-of-s-lst (s-lst)
-    :returns (hash-code integerp)
+  (define get-hash-code-of-s-lst ((s-lst true-listp))
+    :returns (mv (hash-code1 integerp)
+                 (hash-code2 integerp))
     :inline t
-    ;;(loop$ for x in s-lst sum (get-hash-code-of-single-s x))
-    (if (atom s-lst)
+    (mv (ifix (loop$ for x in s-lst sum (get-hash-code-of-single-s x)))
+        ;;(ifix (loop$ for x in s-lst sum (get-hash-code-of-single-s x)))
+        (ifix (loop$ for x in s-lst sum (mod (get-hash-code-of-single-s x) 2)))
+        )
+   #| (if (atom s-lst)
         0
       (+ (get-hash-code-of-single-s (car s-lst))
-         (get-hash-code-of-s-lst (cdr s-lst)))))
+         (get-hash-code-of-s-lst (cdr s-lst))))||#)
 
   (defwarrant get-hash-code-of-s-lst$inline)
 
-  (define get-hash-code-of-s (s)
-    :returns (hash-code integerp)
+  (define get-hash-code-of-s ((s rp-termp))
+    :returns (mv (hash-code1 integerp)
+                 (hash-code2 integerp))
     :inline t
     (case-match s
       (('list . s-lst)
        (get-hash-code-of-s-lst s-lst))
-      (& 0)))
+      (& (mv 0 0))))
 
   (defwarrant get-hash-code-of-s$inline)
 
@@ -184,7 +198,9 @@
     (b* ((c (ex-from-rp/--loose c)))
       (case-match c
         (('c ('quote hash-code) & & &)
-         (ifix hash-code))
+         (if (consp hash-code)
+             (ifix (cdr hash-code))
+           (ifix hash-code)))
         (''0
          0)
         (& (progn$ (hard-error
@@ -195,15 +211,16 @@
 
   (defwarrant get-hash-code-of-single-c$inline)
 
-  (define get-hash-code-of-c-lst (c-lst)
+  (define get-hash-code-of-c-lst ((c-lst true-listp))
     :returns (hash-code integerp)
     :inline t
-    (if (atom c-lst)
+    (ifix (loop$ for x in c-lst sum (floor (get-hash-code-of-single-c x) 2)))
+    #|(if (atom c-lst)
         0
-      (+ (get-hash-code-of-single-c (car c-lst))
-         (get-hash-code-of-c-lst (cdr c-lst)))))
+      (+ (floor (get-hash-code-of-single-c (car c-lst)) 2)
+         (get-hash-code-of-c-lst (cdr c-lst))))||#)
 
-  (define get-hash-code-of-c (c)
+  (define get-hash-code-of-c ((c rp-termp))
     :returns (hash-code integerp)
     :inline t
     (case-match c
@@ -211,16 +228,21 @@
        (get-hash-code-of-c-lst c-lst))
       (& 0)))
 
-  (define calculate-s-hash (pp c)
+  (define calculate-s-hash ((pp rp-termp)
+                            (c rp-termp))
     :returns (hash-code integerp)
-    (+ (calculate-pp-hash pp)
-       (* 2 (get-hash-code-of-c c))))
+    (+ (* 5 (calculate-pp-hash pp))
+       (* 3 (get-hash-code-of-c c))))
 
-  (define calculate-c-hash (s pp c)
-    :returns (hash-code integerp)
-    (+ (get-hash-code-of-s s)
-       (calculate-pp-hash pp)
-       (* 2 (get-hash-code-of-c c)))))
+  (define calculate-c-hash ((s rp-termp)
+                            (pp rp-termp)
+                            (c rp-termp))
+    :returns (hash-code)
+    (b* ((hash-code-base (calculate-s-hash pp c))
+         ((mv s-hash-codes1 s-hash-codes2)
+          (get-hash-code-of-s s)))
+      (cons (+ hash-code-base s-hash-codes1)
+            (+ hash-code-base s-hash-codes2)))))
 
 
 (local
@@ -538,7 +560,9 @@
 
 (progn
   (define pp-lst-subsetp ((pp-lst1 rp-term-listp)
-                          (pp-lst2 rp-term-listp))
+                          (pp-lst2 rp-term-listp)
+                          &key
+                          (pp-flg 't))
     :measure (+ (cons-count pp-lst1)
                 (cons-count pp-lst2))
     :prepwork ((local
@@ -547,17 +571,19 @@
          ((when (atom pp-lst2)) (atom pp-lst1))
          (cur1 (car pp-lst1))
          (cur2 (car pp-lst2))
-         ((mv order equals) (pp-order cur1 cur2)))
+         ((mv order equals) (if pp-flg (pp-order cur1 cur2) (s-order cur1 cur2))))
       (cond (equals
-             (pp-lst-subsetp (cdr pp-lst1) (cdr pp-lst2)))
+             (pp-lst-subsetp (cdr pp-lst1) (cdr pp-lst2) :pp-flg pp-flg))
             (order nil)
-            (t (pp-lst-subsetp pp-lst1 (cdr pp-lst2))))))
+            (t (pp-lst-subsetp pp-lst1 (cdr pp-lst2) :pp-flg pp-flg)))))
 
   (define pp-subsetp ((pp1 rp-termp)
-                      (pp2 rp-termp))
+                      (pp2 rp-termp)
+                      &key
+                      (pp-flg 't))
     (b* ((pp1-lst (list-to-lst pp1))
          (pp2-lst (list-to-lst pp2)))
-      (pp-lst-subsetp pp1-lst pp2-lst))))
+      (pp-lst-subsetp pp1-lst pp2-lst :pp-flg pp-flg))))
 
 
 (progn
@@ -673,7 +699,9 @@
     (case-match term (('-- c1) (mv c1 t)) (& (mv term nil))))
 
   (define ligth-compress-s-c$fix-pp-lst$for-s ((pp1-lst rp-term-listp)
-                                               (pp2-lst rp-term-listp))
+                                               (pp2-lst rp-term-listp)
+                                               &key
+                                               (pp-flg 't))
     :measure (+ (cons-count pp1-lst)
                 (cons-count pp2-lst))
     :prepwork ((local
@@ -705,31 +733,39 @@
                 (t (mv nil nil))))
          ((when changed)
           (b* (((mv pp1-lst-rest &)
-                (ligth-compress-s-c$fix-pp-lst$for-s (cdr pp1-lst) (cdr pp2-lst) )))
+                (ligth-compress-s-c$fix-pp-lst$for-s (cdr pp1-lst) (cdr
+                                               pp2-lst) :pp-flg pp-flg )))
             (mv (cons new-c1 pp1-lst-rest) t)))
-         ((mv pp-order &)
-          (pp-order (ex-from-rp/--loose c1) (ex-from-rp/--loose c2))))
-      (if pp-order
+         ((mv order &)
+          (if pp-flg
+              (pp-order (ex-from-rp/--loose c1) (ex-from-rp/--loose c2))
+            (s-order (ex-from-rp/--loose c1) (ex-from-rp/--loose c2)))))
+      (if order
           (b* (((mv pp1-lst-rest rest-changed)
-                (ligth-compress-s-c$fix-pp-lst$for-s (cdr pp1-lst) pp2-lst )))
+                (ligth-compress-s-c$fix-pp-lst$for-s (cdr pp1-lst) pp2-lst :pp-flg pp-flg )))
             (mv (cons-with-hint c1 pp1-lst-rest pp1-lst) rest-changed))
         (b* (((mv pp1-lst-rest rest-changed)
-              (ligth-compress-s-c$fix-pp-lst$for-s pp1-lst (cdr pp2-lst) )))
+              (ligth-compress-s-c$fix-pp-lst$for-s pp1-lst (cdr pp2-lst)
+                                               :pp-flg pp-flg )))
           (mv pp1-lst-rest rest-changed)))))
 
   (define light-compress-s-c$fix-pp$for-s ((pp1 rp-termp)
-                                           (pp2 rp-termp))
+                                           (pp2 rp-termp)
+                                           &key
+                                           (pp-flg 't))
     :returns (res-pp1 rp-termp :hyp (rp-termp pp1))
     (b* ((pp1-lst (list-to-lst pp1))
          (pp2-lst (list-to-lst pp2))
          ((mv pp1-lst changed)
-          (ligth-compress-s-c$fix-pp-lst$for-s pp1-lst pp2-lst)))
+          (ligth-compress-s-c$fix-pp-lst$for-s pp1-lst pp2-lst :pp-flg pp-flg)))
       (if changed
           (create-list-instance pp1-lst)
         pp1)))
 
   (define light-compress-s-c$pass-pp-lst ((pp1-lst rp-term-listp)
-                                          (pp2-lst rp-term-listp))
+                                          (pp2-lst rp-term-listp)
+                                          &key
+                                          (pp-flg 't))
     :measure (+ (cons-count pp1-lst)
                 (cons-count pp2-lst))
     :prepwork ((local
@@ -759,7 +795,7 @@
          ;;(case-match c1 (('-- c1) (mv c1 t)) (& (mv c1 nil))))
          ((mv c2-abs c2-signed)
           (abs-term c2))
-;(case-match c2 (('-- c2) (mv c2 t)) (& (mv c2 nil))))
+         ;;(case-match c2 (('-- c2) (mv c2 t)) (& (mv c2 nil))))
          ((mv to-pass passable)
           (cond ((and (rp-equal c1-abs c2-abs)
                       (not (equal c1-signed c2-signed)))
@@ -767,21 +803,27 @@
                 (t (mv nil nil))))
          ((when passable)
           (b* (((mv pp1-lst-rest pp2-lst-rest &)
-                (light-compress-s-c$pass-pp-lst (cdr pp1-lst) (cdr pp2-lst))))
+                (light-compress-s-c$pass-pp-lst (cdr pp1-lst) (cdr pp2-lst)
+                                          :pp-flg pp-flg)))
             (mv pp1-lst-rest (cons to-pass pp2-lst-rest) t)))
-         ((mv pp-order &)
-          (pp-order (ex-from-rp/--loose c1-abs) (ex-from-rp/--loose c2-abs))))
-      (if pp-order
+         ((mv order &)
+          (if pp-flg
+              (pp-order (ex-from-rp/--loose c1-abs) (ex-from-rp/--loose
+                                                     c2-abs))
+            (s-order (ex-from-rp/--loose c1-abs) (ex-from-rp/--loose c2-abs)))))
+      (if order
           (b* (((mv pp1-lst-rest pp2-lst-rest rest-changed)
-                (light-compress-s-c$pass-pp-lst (cdr pp1-lst) pp2-lst)))
+                (light-compress-s-c$pass-pp-lst (cdr pp1-lst) pp2-lst :pp-flg pp-flg)))
             (mv (cons-with-hint c1 pp1-lst-rest pp1-lst)
                 pp2-lst-rest rest-changed))
         (b* (((mv pp1-lst-rest pp2-lst-rest rest-changed)
-              (light-compress-s-c$pass-pp-lst pp1-lst (cdr pp2-lst))))
+              (light-compress-s-c$pass-pp-lst pp1-lst (cdr pp2-lst) :pp-flg pp-flg)))
           (mv pp1-lst-rest (cons-with-hint c2 pp2-lst-rest pp2-lst) rest-changed)))))
 
   (define light-compress-s-c$pass-pp ((pp1 rp-termp)
-                                      (pp2 rp-termp))
+                                      (pp2 rp-termp)
+                                      &key
+                                      (pp-flg 't))
     :returns (mv (res-pp1 rp-termp :hyp (rp-termp pp1))
                  (res-pp2 rp-termp :hyp (and (rp-termp pp1)
                                              (rp-termp pp2)))
@@ -789,7 +831,7 @@
     (b* ((pp1-lst (list-to-lst pp1))
          (pp2-lst (list-to-lst pp2))
          ((mv pp1-lst pp2-lst changed)
-          (light-compress-s-c$pass-pp-lst pp1-lst pp2-lst)))
+          (light-compress-s-c$pass-pp-lst pp1-lst pp2-lst :pp-flg pp-flg)))
       (if changed
           (mv (create-list-instance pp1-lst) (create-list-instance pp2-lst) t)
         (mv pp1 pp2 nil))))
@@ -827,9 +869,12 @@
                               ())))))
 
   (define light-compress-s-c-aux ((pp rp-termp)
+                                  (s rp-termp)
                                   (c-arg rp-termp))
     :returns (mv (pp-res rp-termp :hyp (rp-termp pp))
+                 (s-res rp-termp :hyp (rp-termp s))
                  (c-arg-res rp-termp :hyp (and (rp-termp pp)
+                                               (rp-termp s)
                                                (rp-termp c-arg)))
                  (changed booleanp))
     :measure (cons-count c-arg)
@@ -838,23 +883,28 @@
                               o<-chain-2
                               o<-chain)
                              ())))
+    :verify-guards :after-returns
     (case-match c-arg
       (('list single-c)
        (b* ((single-c (ex-from-rp$ single-c))
             ((unless (and (single-c-p single-c)))
-             (mv pp c-arg nil))
+             (mv pp s c-arg nil))
             (pp-arg1 (cadddr single-c))
+            (s-arg1 (caddr single-c))
             (c-arg1 (car (cddddr single-c)))
-            ((mv pp-new pp-arg1 changed)
-             (light-compress-s-c$pass-pp pp pp-arg1))
-            ((unless changed)
-             (mv pp c-arg nil))
-            ((mv pp-arg1 c-arg1 &)
-             (light-compress-s-c-aux pp-arg1 c-arg1)))
-         (mv pp-new `(list (c ',(calculate-c-hash (caddr single-c) pp-arg1 c-arg1)
-                              ,(caddr single-c) ,pp-arg1 ,c-arg1))
+            ((mv pp-new pp-arg1 changed1)
+             (light-compress-s-c$pass-pp pp pp-arg1 :pp-flg t))
+            ((mv s-new s-arg1 changed2)
+             (light-compress-s-c$pass-pp s s-arg1 :pp-flg nil))
+            ((unless (or changed1 changed2))
+             (mv pp s c-arg nil))
+            ((mv pp-arg1 s-arg1 c-arg1 &)
+             (light-compress-s-c-aux pp-arg1 s-arg1 c-arg1)))
+         (mv pp-new s-new
+             `(list (c ',(calculate-c-hash s-arg1 pp-arg1 c-arg1)
+                       ,s-arg1 ,pp-arg1 ,c-arg1))
              t)))
-      (& (mv pp c-arg nil))))
+      (& (mv pp s c-arg nil))))
 
   (define light-compress-s-c ((term rp-termp))
     :prepwork ((local
@@ -868,94 +918,100 @@
            (case-match single-c
              (('c & & c-pp &)
               (b* ((pp (light-compress-s-c$fix-pp$for-s pp c-pp))
-                   ((mv pp c-arg changed)
-                    (light-compress-s-c-aux pp (cadddr term)))
-                   ((Unless changed)
+                   ((mv pp s-res c-arg changed)
+                    (light-compress-s-c-aux pp ''nil (cadddr term)))
+                   ((unless (and changed
+                                 (equal s-res ''nil))) ;; this has to be nil
+                    ;; all the time but to make the proofs easier...
                     term-orig))
                 `(s ',(calculate-s-hash pp c-arg) ,pp ,c-arg)))
              (& term-orig))))
-        (('c & s-arg pp c-arg)
-         (b* (((mv pp c-arg changed)
-               (light-compress-s-c-aux pp c-arg)))
+        (('c & s pp c-arg)
+         (b* (((mv pp s c-arg changed)
+               (light-compress-s-c-aux pp s c-arg)))
            (if changed
-               `(c ',(calculate-c-hash s-arg pp c-arg) ,s-arg ,pp ,c-arg)
+               `(c ',(calculate-c-hash s pp c-arg) ,s ,pp ,c-arg)
              term-orig)))
         (& term-orig))))
 
-  (define case-match-|('s & pp ('list single-c))|
-    (term)
-    :inline t
-    "Used by decompress-s-c"
-    (case-match term
-      (('s & pp ('list single-c))
-       (mv pp single-c t))
-      (& (mv ''nil ''nil nil))))
+  ;; (define case-match-|('s & pp ('list single-c))|
+  ;;   (term)
+  ;;   :inline t
+  ;;   "Used by decompress-s-c"
+  ;;   (case-match term
+  ;;     (('s & pp ('list single-c))
+  ;;      (mv pp single-c t))
+  ;;     (& (mv ''nil ''nil nil))))
 
-  (define case-match-|('c & ''nil pp ('list single-c))| (term)
-    :inline t
-    "Used by decompress-s-c"
-    (case-match term
-      (('c & ''nil pp ('list single-c))
-       (mv pp single-c t))
-      (& (mv ''nil ''nil nil))))
+  ;; (define case-match-|('c & ''nil pp ('list single-c))| (term)
+  ;;   :inline t
+  ;;   "Used by decompress-s-c"
+  ;;   (case-match term
+  ;;     (('c & ''nil pp ('list single-c))
+  ;;      (mv pp single-c t))
+  ;;     (& (mv ''nil ''nil nil))))
 
-  (define case-match-|('c & ''nil pp ''nil)| (term)
-    :inline t
-    "Used by decompress-s-c"
-    (case-match term
-      (('c & ''nil pp ''nil)
-       (mv pp t))
-      (& (mv ''nil nil))))
+  ;; (define case-match-|('c & ''nil pp ''nil)| (term)
+  ;;   :inline t
+  ;;   "Used by decompress-s-c"
+  ;;   (case-match term
+  ;;     (('c & ''nil pp ''nil)
+  ;;      (mv pp t))
+  ;;     (& (mv ''nil nil))))
 
   (define decompress-s-c ((term rp-termp) &key (limit '(expt 2 30)))
     :measure (nfix limit)
     :guard (natp limit)
     :returns (mv (res-term)
-                 (coughed-term))
+                 (coughed-s)
+                 (coughed-pp))
     :verify-guards nil
-    :prepwork ((local
-                (in-theory (enable case-match-|('s & pp ('list single-c))|
-                                   case-match-|('c & ''nil pp ('list single-c))|
-                                   case-match-|('c & ''nil pp ''nil)|))))
-
-    (b* (((when (zp limit)) (mv term ''nil))
+    (b* (((when (zp limit)) (mv term ''nil ''nil))
          (term-orig term)
-         (term (ex-from-rp$ term))
-         ((mv pp single-c match)
-          (case-match-|('s & pp ('list single-c))| term))
-         ((when match)
-          (b* (((mv single-c coughed-pp)
-                (decompress-s-c single-c :limit (1- limit)))
-               (pp (pp-sum-merge pp coughed-pp))
-               (pp (s-fix-args pp))
-               (c (create-list-instance (list single-c))))
-            (mv `(s ',(calculate-s-hash pp c) ,pp ,c)
-                ''nil)))
-         ((mv pp single-c match)
-          (case-match-|('c & ''nil pp ('list single-c))| term))
-         ((when match)
-          (b* (((mv single-c coughed-pp)
-                (decompress-s-c single-c :limit (1- limit)))
-               (pp (pp-sum-merge pp coughed-pp))
-               ((mv pp-coughed pp) (c-fix-pp-args pp ))
-               (c (create-list-instance (list single-c))))
-            (mv `(c ',(calculate-c-hash ''nil pp c) 'nil ,pp ,c)
-                pp-coughed)))
-         ((mv pp match)
-          (case-match-|('c & ''nil pp ''nil)| term))
-         ((when match)
-          (b* (((mv pp-coughed pp) (c-fix-pp-args pp))
-               (c ''nil))
-            (mv `(c ',(calculate-c-hash ''nil pp c) 'nil ,pp ,c)
-                pp-coughed))))
-      (mv term-orig ''nil))
+         (term (ex-from-rp$ term)))
+      (case-match term
+        (('s & pp ('list single-c))
+         (b* (((mv single-c coughed-s coughed-pp)
+               (decompress-s-c single-c :limit (1- limit)))
+              (- (and (not (equal coughed-s ''nil))
+                      (hard-error 'decompress-s-c
+                                  "We do not expect decompress-s-c to cough s
+    terms to s instances yet... ~%" nil)))
+              (pp (pp-sum-merge pp coughed-s));; for proofs...
+              
+              (pp (pp-sum-merge pp coughed-pp))
+              (pp (s-fix-args pp))
+              (c (create-list-instance (list single-c))))
+           (mv `(s ',(calculate-s-hash pp c) ,pp ,c)
+               ''nil
+               ''nil)))
+        (('c & s pp ('list single-c))
+         (b* (((mv single-c coughed-s coughed-pp)
+               (decompress-s-c single-c :limit (1- limit)))
+              (pp (pp-sum-merge pp coughed-pp))
+              ((mv coughed-pp pp) (c-fix-pp-args pp))
+              (s (s-sum-merge s coughed-s))
+              ((mv coughed-s s) (c-fix-s-args s))
+              (c (create-list-instance (list single-c))))
+           (mv `(c ',(calculate-c-hash s pp c) ,s ,pp ,c)
+               coughed-s
+               coughed-pp)))
+        (('c & s pp ''nil)
+         (b* (((mv coughed-pp pp) (c-fix-pp-args pp))
+              ((mv coughed-s s) (c-fix-s-args s))
+              (c ''nil))
+           (mv `(c ',(calculate-c-hash s pp c) ,s ,pp ,c)
+               coughed-s
+               coughed-pp)))
+        (& (mv term-orig ''nil ''nil))))
     ///
 
     (acl2::defret
      rp-termp-of-<fn>
      :hyp (rp-termp term)
      (and (rp-termp res-term)
-          (rp-termp coughed-term)))
+          (rp-termp coughed-pp)
+          (rp-termp coughed-s)))
 
     (verify-guards decompress-s-c-fn)))
 
@@ -1003,32 +1059,38 @@
   (enable-c-pattern1-reduce t))
 
 
-(define c-pattern1-reduce ((s rp-termp)
-                           (pp rp-termp)
-                           (c rp-termp))
+(define c-pattern1-reduce ((s-lst rp-term-listp)
+                           (pp-lst rp-term-listp)
+                           (c-lst rp-term-listp))
   ;; This function is called before forming a single-c instance as (c s pp c).
   ;; It might be possible to compress the c instance.
-  :returns (mv (s-res rp-termp
-                      :hyp (and (rp-termp s)
-                                (rp-termp pp)
-                                (rp-termp c)))
-               (pp-res rp-termp
-                       :hyp (and (rp-termp s)
-                                 (rp-termp pp)
-                                 (rp-termp c)))
-               (c-res rp-termp
-                      :hyp (and (rp-termp s)
-                                (rp-termp pp)
-                                (rp-termp c))))
+  :returns (mv (s-res-lst rp-term-listp
+                          :hyp (and (rp-term-listp s-lst)
+                                    (rp-term-listp pp-lst)
+                                    (rp-term-listp c-lst)))
+               (pp-res-lst rp-term-listp
+                       :hyp (and (rp-term-listp s-lst)
+                                 (rp-term-listp pp-lst)
+                                 (rp-term-listp c-lst)))
+               (c-res-lst rp-term-listp
+                          :hyp (and (rp-term-listp s-lst)
+                                    (rp-term-listp pp-lst)
+                                    (rp-term-listp c-lst))))
   (cond
-   ((not (equal s ''nil)) (mv s pp c))
-   ((not (c-pattern1-reduce-enabled)) (mv s pp c))
+   ;;(s-lst (mv s-lst pp-lst c-lst))
+   ((not (c-pattern1-reduce-enabled)) (mv s-lst pp-lst c-lst))
    (t
-    (case-match c
-      (('list ('c & ''nil c-pp &))
-       (b* (((unless (pp-subsetp pp c-pp)) (mv s pp c))
-            (--pp (negate-list-instance pp))
-            (single-c `(c '0 ,s ,--pp ,c))
+    (case-match c-lst
+      ((('c & c-s c-pp &))
+       (b* (((unless (and (pp-lst-subsetp pp-lst (list-to-lst c-pp))
+                          (pp-lst-subsetp s-lst (list-to-lst c-s))))
+             (mv s-lst pp-lst c-lst))
+            (--pp-lst (negate-lst pp-lst t))
+            (--s-lst (negate-lst s-lst t))
+            (single-c `(c '0
+                          ,(create-list-instance --s-lst)
+                          ,(create-list-instance --pp-lst)
+                          ,(create-list-instance c-lst)))
             (compressed (light-compress-s-c single-c)))
          (case-match compressed
            (('c & ''nil ''nil ('list single-c))
@@ -1036,21 +1098,25 @@
                  ((unless (and valid
                                (equal max 0)
                                (equal min -1)))
-                  (mv s pp c))
-                 ((mv decompressed coughed-pp)
+                  (mv s-lst pp-lst c-lst))
+                 ((mv decompressed coughed-s coughed-pp)
                   (decompress-s-c single-c))
-                 (coughed-pp (pp-sum-merge pp coughed-pp))
-                 ((unless (equal coughed-pp ''nil))
-                  (mv s pp c)))
+                 (coughed-pp-lst (pp-sum-merge-aux pp-lst (list-to-lst
+                                                           coughed-pp)))
+                 (coughed-s-lst (s-sum-merge-aux s-lst (list-to-lst
+                                                           coughed-s)))
+                 ((unless (and (equal coughed-pp-lst nil)
+                               (equal coughed-s-lst nil)))
+                  (mv s-lst pp-lst c-lst)))
               (case-match decompressed
                 (('c & s pp ('list . c-lst)) ;; changed it to this way to prove
                  ;; measure of c-sum-merge with count-c.
-                 (mv s pp `(list . ,c-lst)))
+                 (mv (list-to-lst s) (list-to-lst pp) c-lst))
                 (('c & s pp ''nil)
-                 (mv s pp ''nil))
-                (& (mv s pp c)))))
-           (& (mv s pp c)))))
-      (& (mv s pp c))))))
+                 (mv (list-to-lst s) (list-to-lst pp) nil))
+                (& (mv s-lst pp-lst c-lst)))))
+           (& (mv s-lst pp-lst c-lst)))))
+      (& (mv s-lst pp-lst c-lst))))))
 
 
 (local
@@ -1142,53 +1208,47 @@
 
 
 
-(define c-pattern2-reduce ((pp-lst-coughed rp-term-listp)
-                           (single-c rp-termp))
-  :returns (mv (res-pp-lst-coughed
-                rp-term-listp
-                :hyp (and (rp-term-listp pp-lst-coughed)
-                          (rp-termp single-c))
-                :hints (("Goal"
-                         :use ((:instance and-subsetp-IMPLIES-and-list-intance
-                                          (pp1 (CADDR (CADDDR (EX-FROM-RP
-                                                               SINGLE-C))))
-                                          (pp2 (CADR (CADDDR (EX-FROM-RP
-                                                              SINGLE-C)))))
-                               (:instance and-subsetp-IMPLIES-and-list-intance
-                                          (pp1 (CADDDR (CADDDR (EX-FROM-RP SINGLE-C))))
-                                          (pp2 (CADR (CADDDR (EX-FROM-RP SINGLE-C))))))
-                         :in-theory (e/d () ()))))
-               (res-single-c rp-termp
-                             :hyp
-                             (and (rp-termp single-c))))
-  :verify-guards nil
-  (b* ((single-c-orig single-c)
-       (single-c (ex-from-rp$ single-c)))
-    (case-match single-c
-      (('c & ''nil ('list pp1 pp2 pp3) ''nil)
+(define c-pattern2-reduce ((s-lst rp-term-listp)
+                           (pp-lst rp-term-listp)
+                           (c-lst rp-term-listp))
+  :returns (mv
+            (res-pp-lst rp-term-listp
+                        :hyp (rp-term-listp pp-lst))
+            (reducedp booleanp))
+  
+  :verify-guards :after-returns
+  (b* (((unless (and (not s-lst)
+                     (not c-lst)))
+        (mv nil nil)))
+    (case-match pp-lst
+      ((''1 pp1 pp2 pp3)
        (b* (((unless (or (equal pp1 ''1)
                          (and (and-subsetp pp2 pp1)
                               (and-subsetp pp3 pp1))))
-             (mv pp-lst-coughed single-c-orig))
+             (mv nil nil))
+            ((mv new-pp-lst1 success1) (single-c-to-pp-lst pp1 pp2 pp3))
+            ((mv new-pp-lst2 success2) (single-s-to-pp-lst pp1 pp2 pp3))
+            ((unless (and success1 success2))
+             (mv nil nil)))
+         (mv (pp-sum-merge-aux new-pp-lst1 new-pp-lst2)  t)))
+      ((pp1 pp2 pp3)
+       (b* (((unless (or (equal pp1 ''1)
+                         (and (and-subsetp pp2 pp1)
+                              (and-subsetp pp3 pp1))))
+             (mv nil nil))
             ((mv new-pp-lst success) (single-c-to-pp-lst pp1 pp2 pp3))
             ((unless success)
-             (mv pp-lst-coughed single-c-orig)))
-         (mv (pp-sum-merge-aux new-pp-lst pp-lst-coughed) ''0)))
-      (('c & ''nil ('list pp1 pp2) ''nil)
+             (mv nil nil)))
+         (mv new-pp-lst t)))
+      ((pp1 pp2)
        (b* (((unless (or (equal pp1 ''1)
                          (and (and-subsetp pp2 pp1))))
-             (mv pp-lst-coughed single-c-orig))
+             (mv nil nil))
             ((mv new-pp-lst success) (single-c-to-pp-lst pp1 pp2 ''0))
             ((unless success)
-             (mv pp-lst-coughed single-c-orig)))
-         (mv (pp-sum-merge-aux new-pp-lst
-                               pp-lst-coughed)
-             ''0)))
-      (& (mv pp-lst-coughed single-c-orig))))
-  ///
-  (verify-guards c-pattern2-reduce
-    :hints (("Goal"
-             :in-theory (e/d () ())))))
+             (mv nil nil)))
+         (mv new-pp-lst t)))
+      (& (mv nil nil)))))
 
 
 (defun quoted-listp (lst)
@@ -1209,209 +1269,10 @@
 
 
 
-(define create-c-instance ((s rp-termp)
-                           (pp rp-termp)
-                           (c rp-termp))
-;:inline t
-  :returns (c-res rp-termp :hyp (and (rp-termp pp)
-                                     (rp-termp s)
-                                     (rp-termp c)))
-  (b* (((mv s pp c)
-        (c-pattern1-reduce s pp c)))
-    (cond ((or (and (equal c ''nil)
-                    (equal s ''nil)
-                    (case-match pp (('list ('and-list & &)) t)))
-               (and (equal c ''nil)
-                    (equal pp ''nil)
-                    (case-match s (('list ('s & & &)) t)
-                      (('list ('rp ''bitp &)) t)))
-               (and (equal s ''nil)
-                    (equal pp ''nil)
-                    (case-match c
-                      (('list single-c)
-                       (or (is-rp-bitp single-c)
-                           (is-c-bitp-traverse single-c))))))
-           ''0)
-          ((and (all-quoted-list s)
-                (all-quoted-list pp)
-                (all-quoted-list c))
-           `',(c 0
-                 (unquote-all (list-to-lst s))
-                 (unquote-all (list-to-lst pp))
-                 (unquote-all (list-to-lst c))))
-          (t
-           (b* ((hash-code (calculate-c-hash s pp c)))
-             `(c ',hash-code ,s ,pp ,c))))))
-
 #|(define s-pattern3-success ()
   t)||#
 
 #|(profile 's-pattern3-success)||#
-
-(local
- (defthm is-rp-of-bitp
-   (is-rp `(rp 'bitp ,x))
-   :hints (("Goal"
-            :in-theory (e/d (is-rp) ())))))
-
-(progn
-  (encapsulate
-    (((s-pattern1-reduce-enabled) => *))
-    (local
-     (defun s-pattern1-reduce-enabled ()
-       nil)))
-
-  (defmacro enable-s-pattern1-reduce (enable)
-    (if enable
-        `(defattach  s-pattern1-reduce-enabled return-t)
-      `(defattach  s-pattern1-reduce-enabled return-nil)))
-
-  (enable-s-pattern1-reduce t))
-
-
-(define s-pattern1-reduce ((pp rp-termp)
-                           (c rp-termp))
-  ;; :returns (mv pp c reduced reducedp)
-  ;; Search for (s pp1 (c pp1 rest))
-  ;; which is equivalant to (s (c -pp1 rest))
-  ;; which is created with compress-s-c
-  ;; if the max/min val of (c -pp1 rest) is 0/-1,
-  ;; then reducedp=1 and reduced=(-- (c -pp1 rest))
-  ;; but it is decompressed so reduced=(sum pp1 (-- (c rest)))
-  ;; reduced will be the value returned from create-s-instance right away.
-
-  :returns (mv #|(pp-res rp-termp :hyp (and (rp-termp pp)
-            (rp-termp c)))||#
-            #|(c-res rp-termp :hyp (and (rp-termp pp)
-            (rp-termp c)))||#
-            (reduced rp-termp :hyp (and (rp-termp pp)
-                                        (rp-termp c)))
-            (reducedp booleanp))
-  (b* (((unless (s-pattern1-reduce-enabled))
-        (mv ''0 nil)))
-    (case-match c
-      (('list ('c & ''nil c-pp &))
-       (b* (((unless (pp-subsetp pp c-pp))
-             (mv ''0 nil))
-            (compressed (light-compress-s-c `(s '0 ,pp ,c))))
-         (case-match compressed
-           (('s & ''nil ('list single-c))
-            (b* (((mv max min valid) (get-max-min-val single-c))
-                 ((unless (and valid
-                               (= max 0)
-                               (= min -1)))
-                  (mv ''0 nil))
-                 ((mv res coughed-pp) (decompress-s-c single-c))
-                 (coughed-pp (negate-list-instance coughed-pp)))
-              (mv `(rp 'bitp (c-res 'nil ,coughed-pp (list (-- ,res))))
-                  t)))
-           (& (mv ''0 nil)))))
-      (& (mv ''0 nil)))))
-
-;; (compress-s-c '(s '0 (list c b a) (list (c '0 'nil (list d c a) 'nil))))
-;; (decompress-s-c '(S '0 (LIST B) (LIST (C '0 'NIL (LIST D (-- C) (-- A)) 'NIL))))
-
-
-
-
-
-(define s-pattern2-reduce ((pp rp-termp)
-                           (c rp-termp))
-  :returns (mv (reduced rp-termp :hyp (and (rp-termp pp)
-                                           (rp-termp c)))
-               (reducedp booleanp))
-  (b* (((unless (equal c ''nil))
-        (mv ''0 nil)))
-    (case-match pp
-      (('list pp1 pp2 pp3)
-       (b* (((unless (or (equal pp1 ''1)
-                         (and (and-subsetp pp2 pp1)
-                              (and-subsetp pp3 pp1))))
-             (mv ''0 nil))
-            ((mv new-pp-lst success)
-             (single-s-to-pp-lst pp1 pp2 pp3))
-            ((Unless success)
-             (mv ''0 nil)))
-         (mv `(rp 'bitp (sum-list ,(create-list-instance new-pp-lst))) t)))
-      (('list pp1 pp2)
-       (b* (((unless (or (equal pp1 ''1)
-                         (and (and-subsetp pp2 pp1))))
-             (mv ''0 nil))
-            ((mv new-pp-lst success)
-             (single-s-to-pp-lst pp1 pp2 ''0))
-            ((Unless success)
-             (mv ''0 nil)))
-         (mv `(rp 'bitp (sum-list ,(create-list-instance new-pp-lst))) t)))
-      (& (mv ''0 nil)))))
-
-
-
-(define create-s-instance ((pp rp-termp)
-                           (c rp-termp))
-  :inline t
-  :returns (res rp-termp
-                :hyp (and (rp-termp pp)
-                          (rp-termp c)))
-  (b* (((mv reduced reducedp)
-        (s-pattern1-reduce pp c))
-       ((when reducedp)
-        reduced)
-       ((mv reduced reducedp)
-        (s-pattern2-reduce pp c))
-       ((when reducedp)
-        reduced)
-       )
-    (cond ((and (quotep pp)
-                (quotep c)
-                (consp (cdr pp))
-                (consp (cdr c)))
-           `',(s 0 (unquote pp) (unquote c)))
-          ((and (all-quoted-list pp)
-                (all-quoted-list c))
-           `',(s 0
-                 (unquote-all (list-to-lst pp))
-                 (unquote-all (list-to-lst c))))
-          ((and (equal c ''nil)
-                (case-match pp (('list ('and-list & &)) t)))
-           (cadr pp))
-          ((and (equal pp ''nil)
-                (case-match c
-                  (('list single-c)
-                   (or (is-rp-bitp single-c)))))
-           (cadr c))
-          ((and (equal pp ''nil)
-                (case-match c
-                  (('list single-c)
-                   (is-c-bitp-traverse single-c))))
-           `(rp 'bitp ,(cadr c)))
-          (t
-           `(rp 'bitp (s ',(calculate-s-hash pp c) ,pp ,c))))))
-
-(define swap-c-lsts (c1-lst c2-lst enabled)
-  :inline t
-  :returns (mv (res1 rp-term-listp
-                     :hyp (and (rp-term-listp c1-lst)
-                               (rp-term-listp c2-lst)))
-               (res2 rp-term-listp
-                     :hyp (and (rp-term-listp c1-lst)
-                               (rp-term-listp c2-lst))))
-  (b* (((unless enabled)
-        (mv c1-lst c2-lst))
-       (first-id  (case-match c1-lst
-                    ((('c ('quote hash) . &) . &) hash)
-                    (& 0)))
-       (second-id (case-match c2-lst
-                    ((('c ('quote hash) . &) . &) hash)
-                    (& 0)))
-       (len2 (len c2-lst))
-       (len1 (len c1-lst))
-       (swap (if (= len1 len2)
-                 (> (nfix first-id)
-                    (nfix second-id))
-               (> len1 len2))))
-    (if swap
-        (mv c2-lst c1-lst)
-      (mv c1-lst c2-lst))))
 
 (progn
   (define light-s-of-s-fix-lst ((s-lst rp-term-listp)
@@ -1459,6 +1320,12 @@
          (pp (create-list-instance pp-lst)))
       (mv pp c-lst)))
 
+  (define single-c-try-merge-params-aux-failed ()
+    :enabled t
+    nil)
+
+  (profile 'single-c-try-merge-params-aux-failed)
+  
   (define single-c-try-merge-params-aux ((cur-s rp-termp)
                                          c-hash-code
                                          (s-arg rp-termp)
@@ -1472,8 +1339,11 @@
          (and (equal c-hash-code s-hash-code)
               (b* (((mv pp-arg c-arg-lst)
                     (light-s-of-s-fix s-arg pp-arg c-arg-lst)))
-                (and (equal c-arg-lst (list-to-lst cur-c-arg))
-                     (equal pp-arg cur-pp-arg)))))
+                (or
+                 (and (rp-equal-cnt-subterms c-arg-lst (list-to-lst cur-c-arg) 0)
+                      (rp-equal-cnt pp-arg cur-pp-arg 0))
+                 ;;(single-c-try-merge-params-aux-failed)
+                 ))))
         (&
          (hard-error 'single-c-try-merge-params-aux
                      "Bad form for current s:~p0~%"
@@ -1499,6 +1369,400 @@
          ((when success)
           (mv (cons (car s-lst) rest-s-lst) t)))
       (mv s-lst nil))))
+
+
+(local
+ (defthm is-rp-of-bitp
+   (is-rp `(rp 'bitp ,x))
+   :hints (("Goal"
+            :in-theory (e/d (is-rp) ())))))
+
+(progn
+  (encapsulate
+    (((s-pattern1-reduce-enabled) => *))
+    (local
+     (defun s-pattern1-reduce-enabled ()
+       nil)))
+
+  (defmacro enable-s-pattern1-reduce (enable)
+    (if enable
+        `(defattach  s-pattern1-reduce-enabled return-t)
+      `(defattach  s-pattern1-reduce-enabled return-nil)))
+
+  (enable-s-pattern1-reduce t))
+
+
+(define s-pattern1-reduce ((pp rp-termp)
+                           (c rp-termp))
+  ;; :returns (mv pp c reduced reducedp)
+  ;; Search for (s pp1 (c pp1 rest))
+  ;; which is equivalant to (s (c -pp1 rest))
+  ;; which is created with compress-s-c
+  ;; if the max/min val of (c -pp1 rest) is 0/-1,
+  ;; then reducedp=1 and reduced=(-- (c -pp1 rest))
+  ;; but it is decompressed so reduced=(sum pp1 (-- (c rest)))
+  ;; reduced will be the value returned from create-s-instance right away.
+
+  :returns (mv (reduced-pp-lst rp-term-listp
+                               :hyp (and (rp-termp pp)
+                                         (rp-termp c)))
+               (reduced-c-lst rp-term-listp
+                              :hyp (and (rp-termp pp)
+                                      (rp-termp c)))
+               (reducedp booleanp))
+  (b* (((unless (s-pattern1-reduce-enabled))
+        (mv nil nil nil)))
+    (case-match c
+      (('list ('c & ''nil c-pp &))
+       (b* (((unless (pp-subsetp pp c-pp))
+             (mv nil nil nil))
+            (compressed (light-compress-s-c `(s '0 ,pp ,c))))
+         (case-match compressed
+           (('s & ''nil ('list single-c))
+            (b* (((mv max min valid) (get-max-min-val single-c))
+                 ((unless (and valid
+                               (= max 0)
+                               (= min -1)))
+                  (mv nil nil nil))
+                 ((mv res coughed-s coughed-pp) (decompress-s-c single-c))
+                 ((unless (equal coughed-s ''nil))
+                  (mv nil nil nil))
+                 (coughed-pp (negate-list-instance coughed-pp)))
+              (mv (list-to-lst coughed-pp)
+                  (list `(-- ,res))
+                  t)))
+           (& (mv nil nil nil)))))
+      (& (mv nil nil nil)))))
+
+;; (compress-s-c '(s '0 (list c b a) (list (c '0 'nil (list d c a) 'nil))))
+;; (decompress-s-c '(S '0 (LIST B) (LIST (C '0 'NIL (LIST D (-- C) (-- A)) 'NIL))))
+
+(define s-pattern2-reduce ((pp rp-termp)
+                           (c rp-termp))
+  :returns (mv (reduced-pp-lst rp-term-listp
+                               :hyp (and (rp-termp pp)
+                                         (rp-termp c)))
+               (reducedp booleanp))
+  (b* (((unless (equal c ''nil))
+        (mv nil nil)))
+    (case-match pp
+      (('list ''1 pp1 pp2 pp3)
+       (b* (((unless (or (equal pp1 ''1)
+                         (and (and-subsetp pp2 pp1)
+                              (and-subsetp pp3 pp1))))
+             (mv nil nil))
+            ((mv new-pp-lst success)
+             (single-s-to-pp-lst pp1 pp2 pp3))
+            ((Unless success)
+             (mv nil nil)))
+         (mv (pp-sum-merge-aux (list ''1) (negate-lst new-pp-lst)) t)))
+      (('list pp1 pp2 pp3)
+       (b* (((unless (or (equal pp1 ''1)
+                         (and (and-subsetp pp2 pp1)
+                              (and-subsetp pp3 pp1))))
+             (mv nil nil))
+            ((mv new-pp-lst success)
+             (single-s-to-pp-lst pp1 pp2 pp3))
+            ((Unless success)
+             (mv nil nil)))
+         (mv new-pp-lst t)))
+       ;;(mv `(rp 'bitp (sum-list ,(create-list-instance new-pp-lst))) t)
+      (('list pp1 pp2)
+       (b* (((unless (or (equal pp1 ''1)
+                         (and (and-subsetp pp2 pp1))))
+             (mv nil nil))
+            ((mv new-pp-lst success)
+             (single-s-to-pp-lst pp1 pp2 ''0))
+            ((Unless success)
+             (mv nil nil)))
+         (mv new-pp-lst t)))
+         ;;(mv `(rp 'bitp (sum-list ,(create-list-instance new-pp-lst))) t)))
+      (& (mv nil nil)))))
+
+(progn
+  (encapsulate
+    (((pattern3-reduce-enabled) => *))
+    (local
+     (defun pattern3-reduce-enabled ()
+       nil)))
+
+  (defmacro enable-pattern3-reduce (enable)
+    (if enable
+        `(defattach  pattern3-reduce-enabled return-t)
+      `(defattach  pattern3-reduce-enabled return-nil)))
+
+  (enable-pattern3-reduce nil))
+
+
+(define odd-many-ones (pp-lst)
+  (cond ((atom pp-lst)
+         nil)
+        ((equal (car pp-lst) ''1)
+         (not (odd-many-ones (cdr pp-lst))))
+        (t nil))
+  ///
+  (defthm odd-many-ones-implies-consp
+    (implies (odd-many-ones pp-lst)
+             (and (consp pp-lst)
+                  (equal (car pp-lst) ''1)))
+    :rule-classes :forward-chaining))
+    
+
+(define s-pattern3-reduce ((pp rp-termp)
+                           (c rp-termp))
+  :returns (mv (s-res-lst rp-term-listp
+                          :hyp (and (rp-termp pp)
+                                    (rp-termp c)))
+               (pp-res-lst rp-term-listp
+                           :hyp (and (rp-termp pp)
+                                     (rp-termp c)))
+               (reducedp booleanp))
+  :prepwork
+  ((local
+    (defthm lemma1
+      (implies (rp-term-listp lst)
+               (rp-term-listp (cdr lst))))))
+  
+  (b* (((unless (pattern3-reduce-enabled))
+        (mv nil nil nil))
+       (pp-lst (list-to-lst pp))
+       ((unless (odd-many-ones pp-lst))
+        (mv nil nil nil))
+       (rest-pp-lst (cdr pp-lst))
+       (new-pp (create-list-instance rest-pp-lst))
+       (single-s `(rp 'bitp (s ',(calculate-s-hash new-pp c)
+                               ,new-pp
+                               ,c))))
+    (mv (list `(-- ,single-s))
+        (list ''1)
+        t)))
+
+
+
+
+
+(progn
+  (define single-c-mergeable ((single-c1 rp-termp)
+                              (single-c2 rp-termp))
+    (b* (((when (or (negated-termp single-c1)
+                    (negated-termp single-c2)))
+          nil)
+         ((mv c1-hash-code ?s-arg1 ?pp-arg1 ?c-arg1-lst type1) (get-c-args single-c1))
+         ((mv &            ?s-arg2 ?pp-arg2 ?c-arg2-lst type2) (get-c-args single-c2))
+         ((when (or (not type1) (not type2)))
+          (progn$ (hard-error
+                   'single-c-mergeable
+                   "Unexpected single-c instances.~%single-c1:~p0~%single-c2:~p1~%"
+                   (list (cons #\0 (list type1 single-c1))
+                         (cons #\1 (list type2 single-c2))))
+                 nil))
+         ((unless (case-match s-arg2 (('list . &) t)))
+          nil)
+         ;; search for a merge potential by going through s-lst of the single-c2
+         ;; when a match is found, that s will be removed from the list.
+         ((mv & success)
+          (single-c-try-merge-params (cdr s-arg2)
+                                     c1-hash-code
+                                     s-arg1
+                                     pp-arg1
+                                     c-arg1-lst)))
+      success))
+  (defwarrant single-c-mergeable)
+  
+  (define not-well-merged-c-lst ((c-lst rp-term-listp))
+    :prepwork
+    ((local
+      (in-theory (e/d ( (:definition acl2::apply$-badgep)
+                        (:linear acl2::apply$-badgep-properties . 1)
+                        (:definition subsetp-equal)
+                        (:definition member-equal)
+                        (:rewrite
+                         acl2::member-equal-newvar-components-1))
+                      ()))))
+    (loop$ for x in c-lst when :guard (and (rp-term-listp c-lst)
+                                           (rp-termp x))
+           (loop$ for y in c-lst
+                  when :guard (and (rp-term-listp c-lst)
+                                   (rp-termp y)
+                                   (rp-termp x))
+                  (and
+                   (not (equal x y))
+                   (single-c-mergeable x y))
+                  collect t)
+           collect t)))
+
+
+(define create-s-instance ((pp rp-termp)
+                           (c rp-termp))
+  :inline t
+  :returns (mv (s-res-lst rp-term-listp
+                          :hyp (and (rp-termp pp)
+                                    (rp-termp c)))
+               (pp-res-lst rp-term-listp
+                           :hyp (and (rp-termp pp)
+                                     (rp-termp c)))
+               (c-res-lst rp-term-listp
+                          :hyp (and (rp-termp pp)
+                                    (rp-termp c))))
+  (b* (#|(- (and (not-well-merged-c-lst (list-to-lst c))
+               (hard-error 'create-s-instance
+                           "Mergable c-lst ~p0 ~%"
+                           (list (cons #\0 (list-to-lst c))))))||#
+       
+       ((mv reduced-pp-lst reduced-c-lst reducedp)
+        (s-pattern1-reduce pp c))
+       ((when reducedp)
+        (mv nil reduced-pp-lst reduced-c-lst))
+       ((mv reduced-pp-lst reducedp)
+        (s-pattern2-reduce pp c))
+       ((when reducedp)
+        (mv nil reduced-pp-lst nil))
+       ((mv reduced-s-lst reduced-pp-lst reducedp)
+        (s-pattern3-reduce pp c))
+       ((when reducedp)
+        (mv reduced-s-lst reduced-pp-lst nil))
+       )
+    (cond ((and (quotep pp)
+                (quotep c)
+                (consp (cdr pp))
+                (consp (cdr c)))
+           (mv nil (list `',(s 0 (unquote pp) (unquote c))) nil))
+          ((and (all-quoted-list pp)
+                (all-quoted-list c))
+           (mv nil
+               (list `',(s 0
+                           (unquote-all (list-to-lst pp))
+                           (unquote-all (list-to-lst c))))
+               nil))
+          ((and (equal c ''nil)
+                (case-match pp (('list ('and-list & &)) t)))
+           (mv nil (list (cadr pp)) nil))
+          ((and (equal pp ''nil)
+                (case-match c
+                  (('list single-c)
+                   (or (is-rp-bitp single-c)))))
+           (mv nil nil (list (cadr c))))
+          ((and (equal pp ''nil)
+                (case-match c
+                  (('list single-c)
+                   (is-c-bitp-traverse single-c))))
+           (mv nil nil (list `(rp 'bitp ,(cadr c)))))
+          (t
+           (mv (list `(rp 'bitp (s ',(calculate-s-hash pp c) ,pp ,c)))
+               nil
+               nil)))))
+
+
+
+
+
+(define create-c-instance ((s-lst rp-term-listp)
+                           (pp-lst rp-term-listp)
+                           (c-lst rp-term-listp)
+                           ;;(s-coughed-lst rp-term-listp)
+                           ;;(pp-coughed-lst rp-term-listp)
+                           )
+;:inline t
+  :returns (mv (res-s-lst rp-term-listp
+                          :hyp (and (rp-term-listp s-lst)
+                                    (rp-term-listp pp-lst)
+                                    (rp-term-listp c-lst)
+                                    ;;(rp-term-listp s-coughed-lst)
+                                    ;;(rp-term-listp pp-coughed-lst)
+                                    ))
+               (res-pp-lst rp-term-listp
+                          :hyp (and (rp-term-listp s-lst)
+                                    (rp-term-listp pp-lst)
+                                    (rp-term-listp c-lst)
+                                    ;;(rp-term-listp s-coughed-lst)
+                                    ;;(rp-term-listp pp-coughed-lst)
+                                    ))
+               (res-c-lst rp-term-listp
+                          :hyp (and (rp-term-listp s-lst)
+                                    (rp-term-listp pp-lst)
+                                    (rp-term-listp c-lst)
+                                    ;;(rp-term-listp s-coughed-lst)
+                                    ;;(rp-term-listp pp-coughed-lst)
+                                    )))
+  (b* (#|(- (and (not-well-merged-c-lst c-lst)
+               (hard-error 'create-c-instance
+                           "Mergable c-lst ~p0 ~%"
+                           (list (cons #\0 c-lst)))))||#
+       ((mv s-lst pp-lst c-lst)
+        (c-pattern1-reduce s-lst pp-lst c-lst))
+       ((mv reduced-pp-lst reducedp)
+        (c-pattern2-reduce s-lst pp-lst c-lst))
+       ((when reducedp)
+        (mv nil reduced-pp-lst nil))
+       #|((mv reduced-s-lst reduced-pp-lst reduced-c-lst reducedp)
+        (c-pattern3-reduce s-lst pp-lst c-lst))||#
+       #|((when reducedp)
+        (mv reduced-s-lst reduced-pp-lst reduced-c-lst))||#)
+    (cond ((or (and (equal c-lst nil)
+                    (equal s-lst nil)
+                    (case-match pp-lst
+                      ((('and-list & &)) t)))
+               (and (equal c-lst nil)
+                    (equal pp-lst nil)
+                    (case-match s-lst
+                      ((('s & & &)) t)
+                      ((('rp ''bitp &)) t)))
+               (and (equal s-lst nil)
+                    (equal pp-lst nil)
+                    (case-match c-lst
+                      ((single-c)
+                       (or (is-rp-bitp single-c)
+                           (is-c-bitp-traverse single-c))))))
+           (mv nil nil nil)) 
+          ((and (quoted-listp s-lst)
+                (quoted-listp pp-lst)
+                (quoted-listp c-lst))
+           (b* ((res
+                 `',(c 0
+                       (unquote-all s-lst)
+                       (unquote-all pp-lst)
+                       (unquote-all c-lst))))
+             (if (equal res ''0)
+                 (mv nil nil nil)
+               (mv nil (list res) nil))))
+          (t
+           (b* ((s (create-list-instance s-lst))
+                (pp (create-list-instance pp-lst))
+                (c (create-list-instance c-lst))
+                (hash-code (calculate-c-hash s pp c)))
+             (mv nil nil (list `(c ',hash-code ,s ,pp ,c))))))))
+
+
+
+                              
+
+(define swap-c-lsts (c1-lst c2-lst enabled)
+  :inline t
+  :returns (mv (res1 rp-term-listp
+                     :hyp (and (rp-term-listp c1-lst)
+                               (rp-term-listp c2-lst)))
+               (res2 rp-term-listp
+                     :hyp (and (rp-term-listp c1-lst)
+                               (rp-term-listp c2-lst))))
+  (b* (((unless enabled)
+        (mv c1-lst c2-lst))
+       (first-id  (case-match c1-lst
+                    ((('c ('quote hash) . &) . &) hash)
+                    (& 0)))
+       (second-id (case-match c2-lst
+                    ((('c ('quote hash) . &) . &) hash)
+                    (& 0)))
+       (len2 (len c2-lst))
+       (len1 (len c1-lst))
+       (swap (if (= len1 len2)
+                 (> (nfix first-id)
+                    (nfix second-id))
+               (> len1 len2))))
+    (if swap
+        (mv c2-lst c1-lst)
+      (mv c1-lst c2-lst))))
+
+
 
 (acl2::defines
  count-c
@@ -1627,11 +1891,14 @@
 
    ))
 
-(define negated-termp (term)
-  :inline t
-  (case-match term (('-- &) t)))
 
 (in-theory (enable PP-LST-TO-PP))
+
+
+
+
+
+
 
 (acl2::defines
  c-sum-merge
@@ -1702,25 +1969,42 @@
         (new-s-arg-lst (s-sum-merge-aux (list-to-lst s-arg1)
                                         (s-sum-merge-aux (list-to-lst arg-coughed-s)
                                                          updated-s-arg2-lst)))
-        (new-s-arg (create-list-instance new-s-arg-lst))
-        ((mv coughed-s new-s-arg)
-         (c-fix-s-args new-s-arg))
+        
+        ((mv coughed-s-lst new-s-arg-lst)
+         (c-fix-arg-aux new-s-arg-lst t))
 
         ((mv coughed-pp-lst new-pp-lst)
-         (c-fix-arg-aux-with-cond pp-lst t (clean-pp-args-cond new-s-arg arg-merged-c-lst)))
+         (c-fix-arg-aux-with-cond pp-lst t (clean-pp-args-cond new-s-arg-lst arg-merged-c-lst)))
 
         ;; To-be-coughed c-lst from the args is the coughed-c-lst of the
         ;; new c instance.
-        (merged-single-c (create-c-instance new-s-arg
-                                            (pp-lst-to-pp new-pp-lst)
-                                            (create-list-instance
-                                             arg-merged-c-lst)))
 
-        ((mv coughed-pp-lst merged-single-c)
-         (c-pattern2-reduce coughed-pp-lst merged-single-c))
+        #|((mv new-s-arg-lst new-pp-lst arg-merged-c-lst
+             coughed-s-lst coughed-pp-lst arg-to-be-coughed-c-lst)
+         (c-pattern3-reduce new-s-arg-lst new-pp-lst arg-merged-c-lst
+                            coughed-s-lst coughed-pp-lst arg-to-be-coughed-c-lst))||#
         
-        (produced-c-lst (cons merged-single-c arg-to-be-coughed-c-lst)))
-     (mv coughed-s coughed-pp-lst produced-c-lst t)))
+        ((mv merged-s-lst merged-pp-lst merged-c-lst)
+         (create-c-instance new-s-arg-lst new-pp-lst arg-merged-c-lst))
+
+
+        #|(- (and (subtermp-lst merged-c-lst ''(409630 . 409630))
+               (hard-error 'single-c-try-merge
+                           "arg-s-lst ~p0 arg-pp-lst2 ~p1 arg-c-lst ~p2 ~%"
+                           (list (cons #\0 new-s-arg-lst )
+                                 (cons #\1 new-pp-lst )
+                                 (cons #\2 arg-merged-c-lst)))))||#
+        
+        #|((mv coughed-pp-lst merged-single-c)
+         (c-pattern2-reduce coughed-pp-lst merged-single-c))||#
+
+        (coughed-s-lst (s-sum-merge-aux coughed-s-lst merged-s-lst))
+        (coughed-pp-lst (pp-sum-merge-aux coughed-pp-lst merged-pp-lst))
+        (produced-c-lst (append arg-to-be-coughed-c-lst merged-c-lst)))
+     (mv (create-list-instance coughed-s-lst)
+         coughed-pp-lst
+         produced-c-lst
+         t)))
 
  (define c-sum-merge-lst-aux ((single-c1 rp-termp)
                               (c2-lst rp-term-listp))
@@ -1907,6 +2191,7 @@
             (rp-termp (car x)))))
 
 (define s-of-s-fix-lst ((s-lst rp-term-listp)
+                        (pp-lst rp-term-listp)
                         (c-lst rp-term-listp)
                         &key
                         (limit '(expt 2 30)))
@@ -1916,42 +2201,40 @@
   :measure (nfix limit)
   :verify-guards nil
   (b* (((when (zp limit))
-        (progn$ (hard-error 's-of-s-fix-aux "Limit reached!.." nil)
-                (mv s-lst c-lst)))
-       ((when (atom s-lst)) (mv nil c-lst))
-       ((mv pp-lst new-c-lst) (s-of-s-fix-lst (cdr s-lst) c-lst :limit (1- limit)))
+        (progn$ (hard-error 's-of-s-fix-lst "Limit reached!.." nil)
+                (mv (append pp-lst s-lst) c-lst)))
+       ((when (atom s-lst)) (mv pp-lst c-lst))
+       ((mv pp-lst c-lst) (s-of-s-fix-lst (cdr s-lst) pp-lst c-lst :limit (1- limit)))
        (cur-s (ex-from-rp/-- (car s-lst))))
     (case-match cur-s
       (('s & cur-pp cur-c)
        (b* ((cur-c-lst (list-to-lst cur-c))
             ((mv coughed-s coughed-pp-lst c-lst &)
-             (c-sum-merge cur-c-lst new-c-lst))
+             (c-sum-merge cur-c-lst c-lst))
             (pp-lst (pp-sum-merge-aux coughed-pp-lst pp-lst))
             (pp-lst (pp-sum-merge-aux (list-to-lst cur-pp) pp-lst))
             (coughed-s-lst (list-to-lst coughed-s))
-            ((unless coughed-s-lst)
-             (mv pp-lst c-lst))
-            ((mv rest-pp-lst c-lst)
-             (s-of-s-fix-lst coughed-s-lst c-lst :limit (1- limit))))
-         (mv (pp-sum-merge-aux rest-pp-lst pp-lst) c-lst)))
+            #|((unless coughed-s-lst)
+             (mv pp-lst c-lst))||#
+            ((mv pp-lst c-lst)
+             (s-of-s-fix-lst coughed-s-lst pp-lst c-lst :limit (1- limit))))
+         (mv pp-lst c-lst)))
       (''nil
-       (mv pp-lst new-c-lst))
+       (mv pp-lst c-lst))
       (&
        (progn$ (cw "Unexpected s term ~p0 ~%" cur-s)
-               (hard-error 's-of-s-fix-aux "Read above.." nil)
-               (mv s-lst
-                   ;;(list-to-lst `(binary-append ,cur-s (list . ,pp-lst)))
-
-                   c-lst)))))
+               (hard-error 's-of-s-fix-lst "Read above.." nil)
+               (mv (cons cur-s pp-lst) c-lst)))))
   ///
   (acl2::defret
    rp-term-listp-of-<fn>
    :hyp (and (rp-term-listp s-lst)
+             (rp-term-listp pp-lst)
              (rp-term-listp c-lst))
    (and (rp-term-listp c-res-lst)
         (rp-term-listp pp-res-lst))))
 
-(define s-of-s-fix ((s rp-termp)
+#|(define s-of-s-fix ((s rp-termp)
                     (pp rp-termp)
                     (c-lst rp-term-listp))
   :verify-guards nil
@@ -1964,13 +2247,101 @@
   (b* ((s-lst (list-to-lst s))
        ((when (equal s-lst nil))  (mv pp c-lst))
        ((mv pp-lst c-lst)
-        (s-of-s-fix-lst s-lst c-lst))
+        (s-of-s-fix-lst s-lst (list-to-lst pp) c-lst))
        ;; MAYBE clear c-lst here!
-       (pp-lst (pp-sum-merge-aux (list-to-lst pp) pp-lst))
+       ;;(pp-lst (pp-sum-merge-aux (list-to-lst pp) pp-lst))
        (pp (create-list-instance pp-lst)))
-    (mv pp c-lst)))
+    (mv pp c-lst)))||#
 
 ;;;;;;;
+
+(define c-pattern3-reduce ((s-lst rp-term-listp)
+                           (pp-lst rp-term-listp)
+                           (c-lst rp-term-listp)
+                           (s-coughed-lst rp-term-listp)
+                           (pp-coughed-lst rp-term-listp)
+                           (c-coughed-lst rp-term-listp))
+  :verify-guards nil
+  :returns (mv (res-s-lst rp-term-listp
+                          :hyp (and (rp-term-listp s-lst)
+                                    (rp-term-listp pp-lst)
+                                    (rp-term-listp c-lst)
+                                    (rp-term-listp s-coughed-lst)
+                                    (rp-term-listp pp-coughed-lst)
+                                    (rp-term-listp c-coughed-lst)
+                                    ))
+               (res-pp-lst rp-term-listp
+                           :hyp (and (rp-term-listp s-lst)
+                                     (rp-term-listp pp-lst)
+                                     (rp-term-listp c-lst)
+                                     (rp-term-listp s-coughed-lst)
+                                     (rp-term-listp pp-coughed-lst)
+                                     (rp-term-listp c-coughed-lst)
+                                     ))
+               (res-c-lst rp-term-listp
+                          :hyp (and (rp-term-listp s-lst)
+                                    (rp-term-listp pp-lst)
+                                    (rp-term-listp c-lst)
+                                    (rp-term-listp s-coughed-lst)
+                                    (rp-term-listp pp-coughed-lst)
+                                    (rp-term-listp c-coughed-lst)
+                                    ))
+               (res-s-coughed-lst rp-term-listp
+                                  :hyp (and (rp-term-listp s-lst)
+                                            (rp-term-listp pp-lst)
+                                            (rp-term-listp c-lst)
+                                            (rp-term-listp s-coughed-lst)
+                                            (rp-term-listp pp-coughed-lst)
+                                            (rp-term-listp c-coughed-lst)
+                                            ))
+               (res-pp-coughed-lst rp-term-listp
+                                   :hyp (and (rp-term-listp s-lst)
+                                             (rp-term-listp pp-lst)
+                                             (rp-term-listp c-lst)
+                                             (rp-term-listp s-coughed-lst)
+                                             (rp-term-listp pp-coughed-lst)
+                                             (rp-term-listp c-coughed-lst)
+                                             ))
+               (res-c-coughed-lst rp-term-listp
+                                  :hyp (and (rp-term-listp s-lst)
+                                            (rp-term-listp pp-lst)
+                                            (rp-term-listp c-lst)
+                                            (rp-term-listp s-coughed-lst)
+                                            (rp-term-listp pp-coughed-lst)
+                                            (rp-term-listp c-coughed-lst)
+                                            )))
+  
+  (b* (((when (or (not (pattern3-reduce-enabled))
+                  (not (odd-many-ones pp-lst))))
+        (mv s-lst pp-lst c-lst s-coughed-lst pp-coughed-lst c-coughed-lst))
+
+       (res-s-lst s-lst)
+       (res-pp-lst (cdr pp-lst))
+       (res-c-lst c-lst)
+       
+       
+       ((mv new-pp-lst new-c-lst)
+        (s-of-s-fix-lst s-lst
+                        (cdr pp-lst)
+                        c-lst))
+
+      #| (- (and (not-well-merged-c-lst new-c-lst)
+               (hard-error 'c-pattern3-reduce
+                           "Mergable c-lst ~p0 ~%"
+                           (list (cons #\0 new-c-lst)))))||#
+       
+       ((mv res-s-lst2 res-pp-lst2 res-c-lst2)
+        (create-s-instance (create-list-instance new-pp-lst)
+                           (create-list-instance new-c-lst)))
+
+       (res-s-coughed-lst (s-sum-merge-aux s-coughed-lst res-s-lst2))
+       (res-pp-coughed-lst (pp-sum-merge-aux pp-coughed-lst res-pp-lst2))
+       (res-c-coughed-lst (s-sum-merge-aux c-coughed-lst res-c-lst2)))
+    (mv res-s-lst res-pp-lst res-c-lst
+        res-s-coughed-lst res-pp-coughed-lst res-c-coughed-lst)))
+
+
+;;;;;;;;;
 
 (define quote-all (lst)
   :returns (res rp-term-listp)
@@ -1979,126 +2350,7 @@
     (cons (list 'quote (car lst))
           (quote-all (cdr lst)))))
 
-(local
- (in-theory (disable
-             pp-term-p)))
 
-(define good-4vec-term-p ((term rp-termp))
-  :measure (cons-count term)
-  :hints (("Goal"
-           :in-theory (e/d (measure-lemmas) ())))
-  (b* ((orig term)
-       (term (ex-from-rp term)))
-    (case-match term
-      (('sv::4vec-bitand x y)
-       (and (good-4vec-term-p x)
-            (good-4vec-term-p y)))
-      (('sv::4vec-bitxor x y)
-       (and (good-4vec-term-p x)
-            (good-4vec-term-p y)))
-      (('sv::4vec-bitor x y)
-       (and (good-4vec-term-p x)
-            (good-4vec-term-p y)))
-      (('sv::4vec-? x y z)
-       (and (good-4vec-term-p x)
-            (good-4vec-term-p y)
-            (good-4vec-term-p z)))
-      (('sv::4vec-?* x y z)
-       (and (good-4vec-term-p x)
-            (good-4vec-term-p y)
-            (good-4vec-term-p z)))
-      (('svl::4vec-bitnot$ ''1 x)
-       (and (good-4vec-term-p x)
-            ))
-      (('svl::bits num start size)
-       (and (equal size ''1)
-            (case-match num
-              (('rp ''integerp x)
-               (atom (ex-from-rp x))))
-            (case-match start
-              (('quote x)
-               (natp x)))))
-      (('sv::4vec-fix$inline x)
-       (and (good-4vec-term-p x)))
-      (('sv::3vec-fix x)
-       (and (good-4vec-term-p x)))
-      (& (pp-term-p orig)))))
-
-(define 4vec->pp-term (term)
-  :returns (pp-term)
-  :measure (cons-count term)
-  :guard (and (rp-termp term)
-              (good-4vec-term-p term))
-  :hints (("Goal"
-           :in-theory (e/d (measure-lemmas) ())))
-  :guard-hints (("Goal"
-                 :in-theory (e/d (good-4vec-term-p) ())))
-  (b* ((orig term)
-       (term (ex-from-rp$ term)))
-    (case-match term
-      (('sv::4vec-bitand x y)
-       (b* ((n1 (4vec->pp-term x))
-            (n2 (4vec->pp-term y)))
-         `(binary-and ,n1 ,n2)))
-      (('sv::4vec-bitxor x y)
-       (b* ((n1 (4vec->pp-term x))
-            (n2 (4vec->pp-term y)))
-         `(binary-xor ,n1 ,n2)))
-      (('sv::4vec-bitor x y)
-       (b* ((n1 (4vec->pp-term x))
-            (n2 (4vec->pp-term y)))
-         `(binary-or ,n1 ,n2)))
-      (('sv::4vec-? x y z)
-       (b* ((n1 (4vec->pp-term x))
-            (n2 (4vec->pp-term y))
-            (n3 (4vec->pp-term z)))
-         `(binary-? ,n1 ,n2 ,n3)))
-      (('sv::4vec-?* x y z)
-       (b* ((n1 (4vec->pp-term x))
-            (n2 (4vec->pp-term y))
-            (n3 (4vec->pp-term z)))
-         `(binary-? ,n1 ,n2 ,n3)))
-      (('svl::4vec-bitnot$ ''1 x)
-       `(binary-not ,(4vec->pp-term x)))
-      (('svl::bits num start &)
-       `(bit-of ,num ,start))
-      (('sv::4vec-fix$inline x)
-       (4vec->pp-term x))
-      (('sv::3vec-fix x)
-       (4vec->pp-term x))
-      (& orig)))
-  ///
-
-  (acl2::defret
-   rp-termp-of--<fn>
-   (rp-termp pp-term)
-   :hyp (rp-termp term)
-
-   :hints (("Goal"
-            :induct (4vec->pp-term term)
-            :do-not-induct t
-            :expand ((:free (rest) (RP-TERMP (cons 'BIT-OF rest)))
-                     (:free (rest) (RP-TERMP (cons 'quote rest)))
-                     (:free (rest) (RP-TERMP (cons 'binary-not rest)))
-                     (:free (rest) (RP-TERMP (cons 'binary-and rest)))
-                     (:free (rest) (RP-TERMP (cons 'binary-or rest)))
-                     (:free (rest) (RP-TERMP (cons 'binary-? rest)))
-                     (:free (rest) (RP-TERMP (cons 'binary-xor rest))))
-            :in-theory (e/d () (rp-termp
-                                falist-consistent)))))
-
-  (acl2::defret
-   pp-term-p-of--<fn>
-   :hyp (good-4vec-term-p term)
-   (pp-term-p pp-term)
-   :hints (("Goal"
-            :induct (4vec->pp-term term)
-            :do-not-induct t
-            :expand ((:free (x y) (pp-term-p (cons x y)))
-                     (:free (x y) (is-rp (cons x y))))
-            :in-theory (e/d (good-4vec-term-p
-                             ex-from-rp)
-                            (rp-termp pp-term-p))))))
 
 (local
  (defthm rp-term-listp-of-append
@@ -2132,7 +2384,7 @@
       (cons term-orig acc))
      ((single-s-p term)
       (cons term-orig acc))
-     ((single-c-res-p term)
+     ((single-s-c-res-p term)
       (cons term-orig acc))
      ((sum-list-p term)
       (cons term-orig acc))
@@ -2147,7 +2399,7 @@
         ;; calls ifix for its arguments..
         (cond ((natp x) (append (repeat x ''1) acc))
               (t (append (repeat (- x) ''-1) acc)))))
-     ((good-4vec-term-p term)
+     ((pp-term-p term)
       (cons term-orig acc))
      (t
       (progn$
@@ -2247,10 +2499,10 @@
       (b* ((s (s-sum-merge s (create-list-instance
                               (list term-orig)))))
         (mv s pp-lst c-lst to-be-coughed-c-lst)))
-     ((single-c-res-p abs-term)
+     ((single-s-c-res-p abs-term)
       (b* (((mv s-arg pp-arg c-arg)
             (case-match abs-term
-              (('c-res s-arg pp-arg c-arg) (mv s-arg pp-arg c-arg))
+              (('s-c-res s-arg pp-arg c-arg) (mv s-arg pp-arg c-arg))
               (& (mv ''nil ''nil ''nil))))
            ((mv s-arg pp-arg c-arg-lst)
             (mv (negate-list-instance s-arg negated)
@@ -2283,8 +2535,8 @@
      ((quote-p abs-term)
       (b* ((pp-lst (pp-sum-merge-aux (list term-orig)  pp-lst)))
         (mv s pp-lst c-lst to-be-coughed-c-lst)))
-     ((good-4vec-term-p abs-term)
-      (b* ((abs-term (4vec->pp-term abs-term))
+     ((pp-term-p abs-term)
+      (b* (;;(abs-term (4vec->pp-term abs-term))
            (pp-lst2 (pp-flatten abs-term negated))
            (pp-lst (pp-sum-merge-aux pp-lst pp-lst2)))
         (mv s pp-lst c-lst to-be-coughed-c-lst)))
@@ -2333,7 +2585,7 @@
         (rp-term-listp to-be-coughed-c-lst))))
 
 ;; (progn
-(define well-formed-new-sum ((term rp-termp))
+#|(define well-formed-new-sum ((term rp-termp))
   :returns (res booleanp)
   (or nil
       (case-match term
@@ -2350,7 +2602,7 @@
                   rest-res)
                  #|((case-match x (('d ('rp ''evenpi ('d-sum & & &))) t))
                  rest-res)||#
-                 ((case-match x (('c-res & & &) t))
+                 ((case-match x (('s-c-res & & &) t))
                   rest-res)
                  ((case-match x (('sum-list &) t))
                   rest-res)
@@ -2360,7 +2612,7 @@
                   nil))))
         (('quote x)
          (integer-listp x))
-        (& nil))))
+        (& nil))))||#
 
 (progn
   (define light-pp-term-p ((term rp-termp))
@@ -2456,6 +2708,100 @@
       (and valid
            (quarternaryp res)))))
 
+
+
+
+
+
+#|(acl2::Defines
+ search-for-1
+ :hints (("Goal"
+          :in-theory (e/d (measure-lemmas) ())))
+ (define search-for-1 (term)
+ :measure (cons-count term)                
+  (b* ((term (ex-from-rp term)))
+    (case-match term
+      (('s & pp c)
+       (or (and (consp (list-to-lst pp))
+                (equal (car (list-to-lst pp)) ''1))
+           (search-for-1-lst (list-to-lst c))))
+      (('s-c-res s & c)
+       (or (search-for-1-lst (list-to-lst s))
+           (search-for-1-lst (list-to-lst c))))
+      (('c & s pp c)
+       (or (and (consp (list-to-lst pp))
+                (equal (car (list-to-lst pp)) ''1))
+           (search-for-1-lst (list-to-lst s))
+           (search-for-1-lst (list-to-lst c))))
+      (& nil))))
+ (define search-for-1-lst (lst)
+   :measure (cons-count lst)
+   (if (atom lst)
+       nil
+     (or (search-for-1 (car lst))
+         (search-for-1-lst (cdr lst))))))||#
+
+
+(define create-s-c-res-instance ((s-lst rp-term-listp)
+                                 (pp-lst rp-term-listp)
+                                 (c-lst rp-term-listp)
+                                 (bitp booleanp))
+  :inline t
+  :returns (res rp-termp :hyp (and (rp-term-listp s-lst)
+                                   (rp-term-listp pp-lst)
+                                   (rp-term-listp c-lst)))
+  :guard-hints (("Goal"
+                 :in-theory (e/d (rp-term-listp) ())))
+  (cond ((and (not pp-lst) (not c-lst)
+              (consp s-lst) (not (cdr s-lst))
+              (single-s-p (ex-from-rp$ (car s-lst))))
+         (cond ((and bitp
+                     (not (hide (is-rp (car s-lst)))))
+                `(rp 'bitp ,(car s-lst)))
+               (t (car s-lst))))
+        ((and (not pp-lst) (not s-lst)
+              (consp c-lst) (not (cdr c-lst))
+              (single-c-p (ex-from-rp$ (car c-lst))))
+         (cond ((and bitp
+                     (not (hide (is-rp (car c-lst)))))
+                `(rp 'bitp ,(car c-lst)))
+               (t (car c-lst))))
+        ((and (quoted-listp s-lst)
+              (quoted-listp pp-lst)
+              (quoted-listp c-lst))
+         `',(s-c-res (unquote-all s-lst)
+                     (unquote-all pp-lst)
+                     (unquote-all c-lst)))
+        (t
+         (b* ((term `(s-c-res ,(create-list-instance s-lst)
+                              ,(create-list-instance pp-lst)
+                              ,(create-list-instance c-lst))))
+           (if bitp
+               `(rp 'bitp ,term)
+             term)))))
+
+(define s-spec-meta-aux ((s rp-termp)
+                         (pp-lst rp-term-listp)
+                         (c-lst rp-term-listp))
+  :verify-guards nil
+  :returns (res rp-termp
+                :hyp (and (rp-termp s)
+                          (rp-term-listp pp-lst)
+                          (rp-term-listp c-lst)))
+  (b* (((mv pp-lst c-lst) (s-of-s-fix-lst (list-to-lst s) pp-lst c-lst))
+       (pp-lst (if (clean-pp-args-cond nil c-lst) (s-fix-pp-args-aux pp-lst)
+                 pp-lst))
+       (c-lst (s-fix-pp-args-aux c-lst))
+       (pp (create-list-instance pp-lst))
+       (c (create-list-instance c-lst))
+       ((mv res-s-lst res-pp-lst res-c-lst) (create-s-instance pp c)))
+    (create-s-c-res-instance res-s-lst res-pp-lst res-c-lst t)))
+
+
+
+
+
+
 (define c-spec-meta-aux ((arg-s rp-termp)
                          (arg-pp-lst rp-term-listp)
                          (arg-c-lst rp-term-listp)
@@ -2469,66 +2815,44 @@
   :verify-guards nil
   :prepwork ((local
               (in-theory (disable natp))))
-  (b* (((mv s-coughed arg-s) (c-fix-s-args arg-s))
-       ((mv pp-coughed-lst arg-pp-lst)
-        (c-fix-arg-aux-with-cond arg-pp-lst t  (clean-pp-args-cond arg-s arg-c-lst)))
+  (b* ((arg-s-lst (list-to-lst arg-s))
+       ((mv coughed-s-lst arg-s-lst) (c-fix-arg-aux arg-s-lst t))
 
-       (single-c-term (create-c-instance arg-s
-                                         (create-list-instance arg-pp-lst)
-                                         (create-list-instance arg-c-lst)))
+       ((mv coughed-pp-lst arg-pp-lst2)
+        (c-fix-arg-aux-with-cond arg-pp-lst t (clean-pp-args-cond arg-s-lst arg-c-lst)))
 
-       ((mv pp-coughed-lst single-c-term)
-        (c-pattern2-reduce pp-coughed-lst single-c-term))
+       ;; ((mv arg-s-lst arg-pp-lst2 arg-c-lst
+       ;;      coughed-s-lst coughed-pp-lst to-be-coughed-c-lst)
+       ;;   (c-pattern3-reduce  arg-s-lst arg-pp-lst2 arg-c-lst
+       ;;                       coughed-s-lst coughed-pp-lst to-be-coughed-c-lst))
 
-       (pp-coughed (create-list-instance pp-coughed-lst))
+       
+       ((mv merged-s-lst merged-pp-lst merged-c-lst)
+        (create-c-instance arg-s-lst arg-pp-lst2 arg-c-lst))
+
+       #|(- (and (subtermp-lst merged-c-lst ''(409630 . 409630))
+               (hard-error 'c-spec-meta-aux
+                           "arg-s-lst ~p0 arg-pp-lst2 ~p1 arg-c-lst ~p2 ~%"
+                           (list (cons #\0 arg-s-lst)
+                                 (cons #\1 arg-pp-lst2)
+                                 (cons #\2 arg-c-lst)))))||#
+       
+       (coughed-s-lst (s-sum-merge-aux coughed-s-lst merged-s-lst))
+       (coughed-pp-lst (pp-sum-merge-aux coughed-pp-lst merged-pp-lst))
        
        ((when (not to-be-coughed-c-lst))
-        (cond ((and (equal s-coughed ''nil)
-                    #|(not single-c-from-c-pattern1)||#
-                    (equal pp-coughed ''nil))
-               (if (quotep single-c-term)
-                   single-c-term
-                 (if quarternaryp
-                     `(rp 'bitp ,single-c-term)
-                   single-c-term)))
-              (t
-               (b* ((c-merged-lst  (list single-c-term))
-                    (res `(c-res ,s-coughed ,pp-coughed ,(create-list-instance c-merged-lst))))
-                 (if quarternaryp
-                     `(rp 'bitp ,res)
-                   res)))))
+        (create-s-c-res-instance coughed-s-lst coughed-pp-lst
+                                 merged-c-lst quarternaryp))
+        
+       ((mv s-coughed2 coughed-pp-lst2 merged-c-lst)
+        (c-sum-merge-lst-lst (append to-be-coughed-c-lst merged-c-lst) nil))
 
-       ((mv s-coughed2 coughed-pp-lst c-merged-lst)
-        (c-sum-merge-lst single-c-term to-be-coughed-c-lst ))
+       (coughed-s-lst (s-sum-merge-aux coughed-s-lst (list-to-lst s-coughed2)))
 
-       (s-coughed (s-sum-merge s-coughed s-coughed2))
+       (coughed-pp-lst (pp-sum-merge-aux coughed-pp-lst coughed-pp-lst2))
 
-       (coughed-pp-lst (pp-sum-merge-aux (list-to-lst pp-coughed) coughed-pp-lst))
-       (pp-coughed (pp-lst-to-pp coughed-pp-lst))
-
-       (res `(c-res ,s-coughed ,pp-coughed (list . ,c-merged-lst)))
-       (res (if quarternaryp `(rp 'bitp ,res) res)))
-    res))
-
-(define s-spec-meta-aux ((s rp-termp)
-                         (pp-lst rp-term-listp)
-                         (c-lst rp-term-listp))
-  :verify-guards nil
-  :returns (res rp-termp
-                :hyp (and (rp-termp s)
-                          (rp-term-listp pp-lst)
-                          (rp-term-listp c-lst)))
-  (b* ((pp (pp-lst-to-pp pp-lst))
-       ((mv pp c-lst) (s-of-s-fix s pp c-lst))
-       
-       (pp (if (clean-pp-args-cond ''nil c-lst) (s-fix-args pp) pp))
-
-       #|(- (and (clean-pp-args-cond ''nil c-lst)
-               (not (equal (s-fix-args pp) pp))
-               (cw "pp-orig : ~p0 ~% " pp-orig)))||#
-
-       (c (create-list-instance c-lst))
-       (res (create-s-instance pp c)))
+       (res (create-s-c-res-instance coughed-s-lst coughed-pp-lst merged-c-lst
+                                     quarternaryp)))
     res))
 
 (define s-c-spec-meta ((term rp-termp))
@@ -2552,8 +2876,7 @@
                 (s-res (s-spec-meta-aux s pp-lst c-lst))
                 (c-res (c-spec-meta-aux s pp-lst c-lst
                                         to-be-coughed-c-lst quarternaryp))
-                (res `(cons ,s-res (cons ,c-res 'nil)))
-                )
+                (res `(cons ,s-res (cons ,c-res 'nil))))
              res))
           (('c-s-spec sum)
            (b* (((mv s pp-lst c-lst to-be-coughed-c-lst);;(mv s pp c)
@@ -2636,12 +2959,13 @@
        binary-or
        binary-not
        bit-fix
-       c-res
+       s-c-res
        c
        m2
        f2
        times2
        s
+       pp
        binary-sum
        sv::3vec-fix
        sv::4vec-fix))))
